red_black/Lem.dfy
@@ -1,0 +1,44 @@
+include "Type.dfy"
+include "Property.dfy"
+module Lem {
+  import opened Type
+  import opened Property
+
+  lemma bst_meaning(t:RbTree)
+    requires t.Node? && is_bst(t)
+    ensures !t.left.Node? || t.left.key < t.key
+    ensures !t.right.Node? || t.right.key > t.key
+  {
+    // assert t.left.key in contain(t.left);
+    assert forall x :: x in contain(t.left) ==> x < t.key;
+    //assert t.left.key < t.key;
+
+    //assert t.right.key in contain(t.right);
+    assert forall x :: x in contain(t.right) ==> x > t.key;
+    // assert t.right.key > t.key;
+  }
+  lemma bst_transitivity_right(t:RbTree)
+    requires t.Node? &&t.left.Node? && is_bst(t)
+    ensures forall x :: x in contain (t.left.right)==> x < t.key
+
+  {
+    assert is_bst(t);
+    assert is_bst(t.left);
+    assert is_bst(t.right);
+    assert forall x :: x in contain(t.left.right) ==> x in contain(t.left);
+
+  }
+
+  lemma bst_transitivity_left(t:RbTree)
+    requires t.Node? && t.right.Node? && is_bst(t)
+    ensures forall x :: x in contain (t.right.left)==> x > t.key
+
+  {
+    assert is_bst(t);
+    assert is_bst(t.right);
+    assert is_bst(t.left);
+    assert forall x :: x in contain(t.right.left) ==> x in contain(t.right);
+  }
+
+
+}
