red_black/Type.dfy
@@ -1,0 +1,21 @@
+module Type {
+  // class NodeC {
+  //   var key: int
+  //   var color: bool // true == RED, false == BLACK
+  //   var index: nat
+  //   constructor(k: int, idx: nat) {
+  //     key := k;
+  //     index := idx;
+  //     color := true;
+  //   }
+  // }
+
+  // class RedBlackTree {
+  //   var arr : array<NodeC>
+  // }
+
+  datatype Color = Red | Black
+  datatype RbTree = Null | Node(color: Color, key: int, left: RbTree, right: RbTree)
+}
+
+
